\documentclass[12pt]{article}
\usepackage{amsmath,amssymb}
\DeclareMathOperator{\E}{\mathbb{E}}
\DeclareMathOperator{\HH}{\mathbb{H}}
\usepackage{graphicx}
\usepackage{hyperref}
\usepackage[latin1]{inputenc}

\begin{document}
ex 2.8
\begin{equation}
p(x|z) = \int_{y} p(x,y)dy = \int_{y}h(x,z)g(y,z)dy = h(x,z)\int_{y}g(y,z)dy = h(x,z)C_1
\end{equation}
similarly
\begin{equation}
p(y|z) = g(y,z)C_2
\end{equation}
it remains to show $C = C_1C_2 = 1$
\begin{equation}
1 = \int_{x,y}p(x,y|z) = C\int_{x}p(x|z)dx\int_{y}p(y|z)dy = C 
\end{equation}
ex 2.17
\begin{equation}
\begin{split}
\displaystyle 
\E[min(x,y)] = \int_{y}[\int_{0}^{y}xdx + \int_{y}^{1}ydx]dy = \int_{y}(\frac{y^2}{2} + y(1-y))dy =\\ 
(\frac{y^3}{6} + \frac{y^2}{2} - \frac{y^3}{3}) \biggr\rvert_{0}^{1} = \frac{1}{3}
\end{split}
\end{equation}

ex. 2.10
\begin{equation}
\begin{split}
\displaystyle 
I(X,Y) = \sum_{x,y}p(y)p(x|y)[\log p(x|y) - \log p(x)] = -\HH(X|Y) - \sum_{x,y}p(y)p(x|y)\log p(x) = \\ -\HH(X|Y) - \sum_{x,y}p(x,y)\log p(x) = \HH(X) - \HH(X|Y)
\end{split}
\end{equation}



\end{document}